isabelle/Completeness.thy
@@ -1,5 +1,5 @@
 theory Completeness
-  imports Prover "HOL-Library.BNF_Corec"
+  imports Prover Model "HOL-Library.BNF_Corec"
 begin
 
 section \<open>Completeness of the prover\<close>
@@ -28,22 +28,6 @@ section \<open>Generating countermodels from saturated escape paths\<close>
 
 definition \<open>tree_fms steps \<equiv> \<Union>fms \<in> sset steps. set (fst (fst fms))\<close>
 
-locale Hintikka =
-  fixes H :: \<open>fm set\<close>
-  assumes
-    Basic: \<open>Pre n ts \<in> H \<Longrightarrow> Neg (Pre n ts) \<notin> H\<close> and
-    AlphaDis: \<open>Dis p q \<in> H \<Longrightarrow> p \<in> H \<and> q \<in> H\<close> and
-    AlphaImp: \<open>Imp p q \<in> H \<Longrightarrow> Neg p \<in> H \<and> q \<in> H\<close> and
-    AlphaCon: \<open>Neg (Con p q) \<in> H \<Longrightarrow> Neg p \<in> H \<and> Neg q \<in> H\<close> and
-    BetaCon: \<open>Con p q \<in> H \<Longrightarrow> p \<in> H \<or> q \<in> H\<close> and
-    BetaImp: \<open>Neg (Imp p q) \<in> H \<Longrightarrow> p \<in> H \<or> Neg q \<in> H\<close> and
-    BetaDis: \<open>Neg (Dis p q) \<in> H \<Longrightarrow> Neg p \<in> H \<or> Neg q \<in> H\<close> and
-    GammaExi: \<open>Exi p \<in> H \<Longrightarrow> \<forall>t \<in> \<Union>f \<in> H. set (subtermFm 0 f). sub 0 t p \<in> H\<close> and
-    GammaUni: \<open>Neg (Uni p) \<in> H \<Longrightarrow> \<forall>t \<in> \<Union>f \<in> H. set (subtermFm 0 f). Neg (sub 0 t p) \<in> H\<close> and
-    DeltaUni: \<open>Uni p \<in> H \<Longrightarrow> \<exists>t. sub 0 t p \<in> H\<close> and
-    DeltaExi: \<open>Neg (Exi p) \<in> H \<Longrightarrow> \<exists>t. Neg (sub 0 t p) \<in> H\<close> and
-    Neg: \<open>Neg (Neg p) \<in> H \<Longrightarrow> p \<in> H\<close>
-
 lemma exactly_one_enabled: \<open>\<forall>sequent phase. \<exists>! r. enabled r (sequent, phase)\<close>
   unfolding enabled_def Ex1_def
   using at_least_one_enabled enabled_unique
@@ -71,7 +55,7 @@ proof
     have \<open>\<exists>s \<in> sset steps. enabled Basic (fst s)\<close>
       sorry
     show False
-      sorry 
+      sorry
   qed
 next
   fix p q
@@ -116,22 +100,22 @@ next
 next
   fix p
   assume \<open>Exi p \<in> tree_fms steps\<close>
-  show \<open>\<forall>t\<in>\<Union>f \<in> tree_fms steps. set (subtermFm 0 f). sub 0 t p \<in> tree_fms steps\<close>
+  show \<open>\<forall>t\<in>\<Union>f \<in> tree_fms steps. set (subtermFm f). sub 0 t p \<in> tree_fms steps\<close>
     sorry
 next
   fix p
   assume \<open>Neg (Uni p) \<in> tree_fms steps\<close>
-  show \<open>\<forall>t\<in>\<Union>f \<in> tree_fms steps. set (subtermFm 0 f). Neg (sub 0 t p) \<in> tree_fms steps\<close>
+  show \<open>\<forall>t\<in>\<Union>f \<in> tree_fms steps. set (subtermFm f). Neg (sub 0 t p) \<in> tree_fms steps\<close>
     sorry
 next
   fix p
   assume \<open>Uni p \<in> tree_fms steps\<close>
-  show \<open>\<exists>t. sub 0 t p \<in> tree_fms steps\<close>
+  show \<open>\<exists>t \<in> terms (tree_fms steps). sub 0 t p \<in> tree_fms steps\<close>
     sorry
 next
   fix p
   assume \<open>Neg (Exi p) \<in> tree_fms steps\<close>
-  show \<open>\<exists>t. Neg (sub 0 t p) \<in> tree_fms steps\<close>
+  show \<open>\<exists>t \<in> terms (tree_fms steps). Neg (sub 0 t p) \<in> tree_fms steps\<close>
     sorry
 next
   fix p
@@ -140,242 +124,9 @@ next
     sorry
 qed
 
-datatype htm = HFun nat \<open>htm list\<close>
-
-fun tm_to_htm :: \<open>tm \<Rightarrow> htm\<close> where
-  \<open>tm_to_htm (Var _) = undefined\<close>
-| \<open>tm_to_htm (Fun n ts) = HFun n (map tm_to_htm ts)\<close>
-
-fun htm_to_tm :: \<open>htm \<Rightarrow> tm\<close> where
-  \<open>htm_to_tm (HFun n hts) = Fun n (map htm_to_tm hts)\<close>
-
-
-lemma \<open>tm_to_htm (htm_to_tm t) = t\<close>
-  sorry  
-
-lemma
-  assumes \<open>closedt t\<close>
-  shows \<open>htm_to_tm (tm_to_htm t) = t\<close>
-  sorry
-
-abbreviation (input) \<open>sat S n ts \<equiv> Neg (Pre n ts) \<in> S\<close>
-
-lemma semantics_id [simp]:
-  \<open>semantics_term Var Fun t = t\<close>
-  \<open>semantics_list Var Fun ts = ts\<close>
-  by (induct t and ts rule: semantics_term.induct semantics_list.induct) simp_all
-
-lemma size_sub [simp]: \<open>size (sub i t p) = size p\<close>
-  by (induct p arbitrary: i t) auto
-
-lemma
-  assumes
-    \<open>\<forall>e. \<forall>t \<in> {Fun i []} \<union> set (subtermFm 0 p). semantics e f g (sub 0 t p)\<close>
-    \<open>i \<notin> params p\<close>
-  shows \<open>semantics e f g (sub 0 t p)\<close>
-proof (cases \<open>t \<in> set (subtermFm 0 p)\<close>)
-  case True
-  then show ?thesis
-    using assms by blast
-next
-  case False
-  let ?x = \<open>semantics_term e f t\<close>
-  let ?y = \<open>f i []\<close>
-
-  (* t = f(g(a)) *)
-
-  have \<open>semantics (SeCaV.shift e 0 ?y) f g p\<close>
-    using assms by simp
-  then have \<open>\<forall>x. semantics (SeCaV.shift e 0 x) f g p\<close>
-    using \<open>i \<notin> params p\<close> sorry
-  then have \<open>semantics (SeCaV.shift e 0 ?x) f g p\<close>
-    by simp
-  then show ?thesis
-    using subst_lemma by simp
-qed
-
-lemma hintikka_counter_model:
-  assumes \<open>Hintikka S\<close>
-  shows \<open>(p \<in> S \<longrightarrow> \<not> semantics Var Fun (sat S) p) \<and> (Neg p \<in> S \<longrightarrow> semantics Var Fun (sat S) p)\<close>
-proof (induct p rule: wf_induct [where r=\<open>measure size\<close>])
-  case 1
-  then show ?case ..
-next
-  fix x
-  assume wf: \<open>\<forall>q. (q, x) \<in> measure size \<longrightarrow>
-      (q \<in> S \<longrightarrow> \<not> semantics Var Fun (sat S) q) \<and>
-      (Neg q \<in> S \<longrightarrow> semantics Var Fun (sat S) q)\<close>
-
-  show \<open>(x \<in> S \<longrightarrow> \<not> semantics Var Fun (sat S) x) \<and>
-        (Neg x \<in> S \<longrightarrow> semantics Var Fun (sat S) x)\<close>
-  proof (cases x)
-    case (Pre n ts)
-    show ?thesis
-    proof (intro conjI impI)
-      assume \<open>x \<in> S\<close>
-      then have \<open>Neg (Pre n ts) \<notin> S\<close>
-        using assms Pre Hintikka.Basic by blast
-      then show \<open>\<not> semantics Var Fun (sat S) x\<close>
-        using Pre by simp
-    next
-      assume \<open>Neg x \<in> S\<close>
-      then have \<open>sat S n ts\<close>
-        using assms Pre Hintikka.Basic by blast
-      then show \<open>semantics Var Fun (sat S) x\<close>
-        using Pre by simp
-    qed
-  next
-    case (Imp p q)
-    show ?thesis
-    proof (intro conjI impI)
-      assume \<open>x \<in> S\<close>
-      then have \<open>Neg p \<in> S\<close> \<open>q \<in> S\<close>
-        using Imp assms Hintikka.AlphaImp by blast+
-      then show \<open>\<not> semantics Var Fun (sat S) x\<close>
-        using wf Imp by fastforce
-    next
-      assume \<open>Neg x \<in> S\<close>
-      then have \<open>p \<in> S \<or> Neg q \<in> S\<close>
-        using Imp assms Hintikka.BetaImp by blast
-      then show \<open>semantics Var Fun (sat S) x\<close>
-        using wf Imp by fastforce
-    qed
-  next
-    case (Dis p q)
-    show ?thesis
-    proof (intro conjI impI)
-      assume \<open>x \<in> S\<close>
-      then have \<open>p \<in> S\<close> \<open>q \<in> S\<close>
-        using Dis assms Hintikka.AlphaDis by blast+
-      then show \<open>\<not> semantics Var Fun (sat S) x\<close>
-        using wf Dis by fastforce
-    next
-      assume \<open>Neg x \<in> S\<close>
-      then have \<open>Neg p \<in> S \<or> Neg q \<in> S\<close>
-        using Dis assms Hintikka.BetaDis by blast
-      then show \<open>semantics Var Fun (sat S) x\<close>
-        using wf Dis by fastforce
-    qed
-  next
-    case (Con p q)
-    show ?thesis
-    proof (intro conjI impI)
-      assume \<open>x \<in> S\<close>
-      then have \<open>p \<in> S \<or> q \<in> S\<close>
-        using Con assms Hintikka.BetaCon by blast
-      then show \<open>\<not> semantics Var Fun (sat S) x\<close>
-        using wf Con by fastforce
-    next
-      assume \<open>Neg x \<in> S\<close>
-      then have \<open>Neg p \<in> S\<close> \<open>Neg q \<in> S\<close>
-        using Con assms Hintikka.AlphaCon by blast+
-      then show \<open>semantics Var Fun (sat S) x\<close>
-        using wf Con by fastforce
-    qed
-  next
-    case (Exi p)
-    show ?thesis
-    proof (intro conjI impI)
-      assume \<open>x \<in> S\<close>
-      then have \<open>\<forall>t \<in> \<Union>f \<in> S. set (subtermFm 0 f). sub 0 t p \<in> S\<close>
-        using Exi assms Hintikka.GammaExi by blast
-      then have \<open>\<forall>t \<in> \<Union>f \<in> S. set (subtermFm 0 f). \<not> semantics Var Fun (sat S) (sub 0 t p)\<close>
-        using wf Exi size_sub
-        by (metis (no_types, lifting) add.right_neutral add_Suc_right fm.size(12) in_measure lessI)
-      (* NEW THOUGHTS: Need to restrict the model so that the universe only contains
-            terms that occur in S.
-            We cannot do this easily with the Isabelle logic.
-            Maybe we can define a semantics a la FEval here:
-              https://www.isa-afp.org/browser_info/current/AFP/Verified-Prover/Prover.html *)
-
-      (* Assume formula is closed and be arbitrary over e *)    
-
-      (* Need a lemma that proves that quantifying over Fun 0 [] and the subterms is enough
-         to generalize to all terms *)
-
-      (* e :: nat \<Rightarrow> {t :: tm. t \<in> \<Union>f \<in> H. set (subtermFm 0 f)}
-
-          e S
-         (f S) n ts : 'a
-
-          datatype htm = HFun nat htm list | Other
-          if Fun n ts \<in> S then HFun n ts else Other
-
-          f :: filter
-
-
-          Sig at t er en subterm af S.
-          Så f t = t og det holder induktivt.
-
-          Sig at t ikke er en subterm af S.
-          Så f t = Fun 0 []
-          Så skal vi vise \<not> semantics Var f (sat S) (sub 0 (Fun 0 []) p)
-            Hvordan gør vi det?
-       *)
-      have \<open>\<forall>t. \<not> semantics Var Fun (sat S) (sub 0 t p)\<close>
-        sorry
-      then have \<open>\<forall>t. \<not> semantics (SeCaV.shift Var 0 t) Fun (sat S) p\<close>
-        using subst_lemma by simp
-      then show \<open>\<not> semantics Var Fun (sat S) x\<close>
-        using Exi by simp
-    next
-      assume \<open>Neg x \<in> S\<close>
-      then obtain t where \<open>Neg (sub 0 t p) \<in> S\<close>
-        using Exi assms Hintikka.DeltaExi by blast
-      then have \<open>semantics Var Fun (sat S) (sub 0 t p)\<close>
-        using wf Exi size_sub
-        by (metis Nat.add_0_right add_Suc_right fm.size(12) in_measure less_Suc_eq)
-      then show \<open>semantics Var Fun (sat S) x\<close>
-        using wf Exi by fastforce
-    qed
-  next
-    case (Uni p)
-    show ?thesis
-    proof (intro conjI impI)
-      assume \<open>x \<in> S\<close>
-      then obtain t where \<open>sub 0 t p \<in> S\<close>
-        using Uni assms Hintikka.DeltaUni by blast
-      then have \<open>\<not> semantics Var Fun (sat S) (sub 0 t p)\<close>
-        using wf Uni size_sub
-        by (metis Nat.add_0_right add_Suc_right fm.size(13) in_measure less_Suc_eq)
-      then show \<open>\<not> semantics Var Fun (sat S) x\<close>
-        using Uni by fastforce
-    next
-      assume \<open>Neg x \<in> S\<close>
-      then have \<open>\<forall>t \<in> \<Union>f \<in> S. set (subtermFm 0 f). Neg (sub 0 t p) \<in> S\<close>
-        using Uni assms Hintikka.GammaUni by blast
-      then have \<open>\<forall>t \<in> \<Union>f \<in> S. set (subtermFm 0 f). semantics Var Fun (sat S) (sub 0 t p)\<close>
-        using wf Uni size_sub
-        by (metis (no_types, lifting) add.right_neutral add_Suc_right fm.size(13) in_measure lessI)
-
-(* SEE ABOVE *)
-      have \<open>\<forall>t. semantics Var Fun (sat S) (sub 0 t p)\<close>
-        sorry
-      then have \<open>\<forall>t. semantics (SeCaV.shift Var 0 t) Fun (sat S) p\<close>
-        using subst_lemma by simp
-      then show \<open>semantics Var Fun (sat S) x\<close>
-        using wf Uni by fastforce
-    qed
-  next
-    case (Neg p)
-    show ?thesis
-    proof (intro conjI impI)
-      assume \<open>x \<in> S\<close>
-      then show \<open>\<not> semantics Var Fun (sat S) x\<close>
-        using wf Neg by fastforce
-    next
-      assume \<open>Neg x \<in> S\<close>
-      then have \<open>p \<in> S\<close>
-        using Neg assms Hintikka.Neg by blast
-      then show \<open>semantics Var Fun (sat S) x\<close>
-        using wf Neg by fastforce
-    qed
-  qed
-qed
-
 text \<open>We need some lemmas to prove our main theorem\<close>
 lemma epath_countermodel:
-  assumes \<open>\<exists> steps. fst (fst (shd steps)) = [p] \<and> epath steps \<and> Saturated steps\<close>
+  assumes \<open>\<exists> steps. fst (fst (shd steps)) = [p] \<and> epath steps \<and> Saturated steps\<close> \<open>closed 0 p\<close>
   shows \<open>\<exists>(e :: nat \<Rightarrow> tm) f g . \<not> (semantics e f g p)\<close>
 proof (rule ccontr)
   assume \<open>\<nexists>(e :: nat \<Rightarrow> tm) f g. \<not> semantics e f g p\<close>
@@ -392,7 +143,7 @@ proof (rule ccontr)
     moreover have \<open>p \<in> tree_fms steps\<close>
       using steps shd_sset unfolding tree_fms_def by force
     then have \<open>\<exists>(e :: nat \<Rightarrow> tm) f g . \<not> semantics e f g p\<close>
-      using calculation(2) hintikka_counter_model steps by blast
+      using calculation(2) hintikka_counter_model assms(2) steps sorry (* by blast *)
     ultimately show \<open>False\<close>
       by blast
   qed
@@ -405,21 +156,21 @@ lemma epath_lem:
   using assms(2) epath_prover_completeness t_def by blast
 
 lemma epath_contr:
-  assumes \<open>\<tturnstile> [p]\<close>
+  assumes \<open>\<tturnstile> [p]\<close> \<open>closed 0 p\<close>
   shows \<open>\<nexists> steps. fst (fst (shd steps)) = [p] \<and> epath steps \<and> Saturated steps\<close>
 proof (rule ccontr, simp)
   show \<open>\<exists> steps. epath steps \<and> fst (fst (shd steps)) = [p] \<and> Saturated steps \<Longrightarrow> False\<close>
   proof -
     assume ep: \<open>\<exists> steps. epath steps \<and> fst (fst (shd steps)) = [p] \<and> Saturated steps\<close>
     have \<open>\<exists>(e :: nat \<Rightarrow> tm) f g . \<not> (semantics e f g p)\<close>
-      using ep epath_countermodel by blast
+      using ep epath_countermodel assms(2) by blast
     with assms show False using sound by fastforce
   qed
 qed
 
 text \<open>Finally, we arrive at the main theorem\<close>
 theorem completeness:
-  assumes \<open>\<tturnstile> [p]\<close>
+  assumes \<open>\<tturnstile> [p]\<close> \<open>closed 0 p\<close>
   defines \<open>t \<equiv> secavProver [p]\<close>
   shows \<open>fst (fst (root t)) = [p] \<and> wf t \<and> tfinite t\<close>
   by (simp add: assms epath_contr epath_lem epath_prover_completeness)
